ind-cca panic free

libcrux-ml-kem/proofs/fstar/extraction/Libcrux_ml_kem.Ind_cca.fsti
@@ -196,6 +196,8 @@ let impl: t_Variant t_MlKem =
       out
   }
 
+#push-options "--z3rlimit 1234"
+
 val decapsulate
       (v_K v_SECRET_KEY_SIZE v_CPA_SECRET_KEY_SIZE v_PUBLIC_KEY_SIZE v_CIPHERTEXT_SIZE v_T_AS_NTT_ENCODED_SIZE v_C1_SIZE v_C2_SIZE v_VECTOR_U_COMPRESSION_FACTOR v_VECTOR_V_COMPRESSION_FACTOR v_C1_BLOCK_SIZE v_ETA1 v_ETA1_RANDOMNESS_SIZE v_ETA2 v_ETA2_RANDOMNESS_SIZE v_IMPLICIT_REJECTION_HASH_INPUT_SIZE:
           usize)
@@ -220,7 +222,12 @@ val decapsulate
         v_ETA2 == Spec.MLKEM.v_ETA2 v_K /\
         v_ETA2_RANDOMNESS_SIZE == Spec.MLKEM.v_ETA2_RANDOMNESS_SIZE v_K /\
         v_IMPLICIT_REJECTION_HASH_INPUT_SIZE == Spec.MLKEM.v_IMPLICIT_REJECTION_HASH_INPUT_SIZE v_K)
-      (fun _ -> Prims.l_True)
+      (ensures
+        fun result ->
+          let result:t_Array u8 (sz 32) = result in
+          result == Spec.MLKEM.ind_cca_decapsulate v_K private_key.f_value ciphertext.f_value)
+
+#pop-options
 
 val encapsulate
       (v_K v_CIPHERTEXT_SIZE v_PUBLIC_KEY_SIZE v_T_AS_NTT_ENCODED_SIZE v_C1_SIZE v_C2_SIZE v_VECTOR_U_COMPRESSION_FACTOR v_VECTOR_V_COMPRESSION_FACTOR v_C1_BLOCK_SIZE v_ETA1 v_ETA1_RANDOMNESS_SIZE v_ETA2 v_ETA2_RANDOMNESS_SIZE:
