libcrux-ml-kem/proofs/fstar/extraction/Libcrux_ml_kem.Ind_cca.fst
@@ -309,16 +309,20 @@ let decapsulate
       shared_secret
       ciphertext
   in
-  Libcrux_ml_kem.Constant_time_ops.compare_ciphertexts_select_shared_secret_in_constant_time (Core.Convert.f_as_ref
-        #(Libcrux_ml_kem.Types.t_MlKemCiphertext v_CIPHERTEXT_SIZE)
-        #(t_Slice u8)
-        #FStar.Tactics.Typeclasses.solve
-        ciphertext
-      <:
-      t_Slice u8)
-    (Rust_primitives.unsize expected_ciphertext <: t_Slice u8)
-    (Rust_primitives.unsize shared_secret <: t_Slice u8)
-    (Rust_primitives.unsize implicit_rejection_shared_secret <: t_Slice u8)
+  let shared_secret:t_Array u8 (sz 32) =
+    Libcrux_ml_kem.Constant_time_ops.compare_ciphertexts_select_shared_secret_in_constant_time (Core.Convert.f_as_ref
+          #(Libcrux_ml_kem.Types.t_MlKemCiphertext v_CIPHERTEXT_SIZE)
+          #(t_Slice u8)
+          #FStar.Tactics.Typeclasses.solve
+          ciphertext
+        <:
+        t_Slice u8)
+      (Rust_primitives.unsize expected_ciphertext <: t_Slice u8)
+      (Rust_primitives.unsize shared_secret <: t_Slice u8)
+      (Rust_primitives.unsize implicit_rejection_shared_secret <: t_Slice u8)
+  in
+  let _:Prims.unit = admit () in
+  shared_secret
 
 let encapsulate
       (v_K v_CIPHERTEXT_SIZE v_PUBLIC_KEY_SIZE v_T_AS_NTT_ENCODED_SIZE v_C1_SIZE v_C2_SIZE v_VECTOR_U_COMPRESSION_FACTOR v_VECTOR_V_COMPRESSION_FACTOR v_C1_BLOCK_SIZE v_ETA1 v_ETA1_RANDOMNESS_SIZE v_ETA2 v_ETA2_RANDOMNESS_SIZE:
